\input{setup}

\title{Exercise 3, Nano Life Science}
\author{Viljar Femoen}
\input{commands}

\begin{document}
\maketitle
\section*{Task 1}

The Navier-Stokes equation states 
\begin{equation*}
    \pde{\vec{v}}{t} + \left(\vec{v} \cdot \nabla\right)\vec{v} = - \frac{1}{\rho}\nabla p + \frac{\eta}{\rho}\nabla^2\vec{v}.
\end{equation*}

In our case, $\vec{v} = v\hat{z}$, and we have cylindrical symmetry, meaning $\left(\vec{v} \cdot \nabla\right)\vec{v} =  0.$
Furthermore, $\nabla p = \frac{\Delta p}{l}\hat{z}$, and we assume steady-state, i.e. $\pde{v}{t} = 0$, which means we can write the above equation as
\begin{equation*}
    \nabla^2\vec{v} = \frac{\Delta p}{l\eta}\hat{z}.
\end{equation*}

With cylindrical coordinates, the left-hand-side evaluates to

\begin{equation*}
    \nabla^2 v_z\hat{z} = \frac{1}{r}\pde{}{r}\left(r\pde{v_z}{r}\right)\hat{z}. 
\end{equation*}

Using the chain rule, we arrive at the following ODE:

\begin{equation*}
    \pde[2]{v_z}{r} + \frac{1}{r}\pde{v_z}{r} = \frac{\Delta p}{l\eta}.
\end{equation*}

Laplace transforming this, we arrive at 

\begin{equation*}
    -\frac{d}{ds}\left(s^2\tilde{v}_z - sv_z(0) + \pde{v_z}{r}_{r = 0}\right) + s\tilde{v}_z - v_z(0) = \frac{\Delta p}{l\eta s^2}.
\end{equation*}

We have the no-slip condition, i.e. $v_z(0) = 0$, and as such the above equation becomes

\begin{align*}
    \tilde{v}_z + s\ode{\tilde{v}_z}{s} &= -\frac{\Delta p}{l\eta s^3} \\
    \ode{}{s}\left(s\tilde{v}_z\right) &= -\frac{\Delta p}{l\eta s^3} \\
    s\tilde{v}_z &= c_1 - \frac{\Delta p}{2l\eta s^2} \\
    \tilde{v}_z &= \frac{c_1}{s} - \frac{\Delta p}{2l\eta s^3},
\end{align*}
for an arbitrary real constant $c_1$. Inverse laplace transforming back to real space, we arrive at

\begin{equation*}
    v_z(r) = c_1 - \frac{\Delta pr^2}{4l\eta}.
\end{equation*}

Re-applying the no-slip condition, we get the following equation for $c_1$:

\begin{equation*}
    0 = c_1 - \frac{\Delta p\left(\frac{d}{2}\right)^2}{4l\eta},
\end{equation*}
which finally lets us write
\begin{equation*}
    v_z(r) = \frac{\Delta p}{4l\eta}\left(\frac{d^2}{4} - r^2\right).
\end{equation*}

$\left<v\right>_r$ is given by

\begin{equation*}
    \int_{-\infty}^\infty rv_z(r)dr = \frac{\Delta p}{4l\eta}\int_0^\frac{d}{2} r\left(\frac{d^2}{4} - r^2\right)dr = \frac{\Delta p d^2}{24l\eta}.
\end{equation*}

The maximum velocity, $v_\text{max} = v(r = 0) = \frac{\Delta p d^2}{16l\eta}$, is a factor $\frac{d^2}{16}$ away from the average. 
Therefore, the smaller the channel, the smaller the relative difference between the max and the average will be.

The volumetric flow rate is given by

\begin{equation*}
    Q = \iint v dA = \int_0^{2\pi}\int_0^\frac{d}{2} v rdrd\theta 
    = \frac{\Delta p}{4l\eta}\int_0^{2\pi} \int_0^\frac{d}{2} r\left(\frac{d^2}{4} - r^2\right)drd\theta 
    = \frac{\pi\Delta p d^4}{128l\eta},
\end{equation*}
which was to be shown. 

\section*{Task 2}

We know

To compute $\left<x^2\right>$, one needs to evaluate the integral

\begin{equation*}
    \int_{-\infty}^\infty x^2 p(x) dx = \int_{-\infty}^\infty x^2 e^{-\beta k\frac{x^2}{2}} dx = \sqrt{\frac{2\pi}{k^3\beta^3}},
\end{equation*}

and normalize, i.e. divide by 

\begin{equation*}
    \int_{-\infty}^\infty p(x) dx = \sqrt{\frac{2\pi}{k\beta}}.
\end{equation*}

$p(x)$ is the probability of finding a particle at position $x$, and is given by the Bolzmann distribution: $e^{-\beta U(x)}$.

Rearranging, we get

\begin{eqnarray}
    k = \frac{k_bT}{\left<x^2\right>},
\end{eqnarray}
which was to be shown.
\end{document}